Optativas/VFS/practicas/Clase7.Imp.fst
@@ -78,27 +78,78 @@ type runsto : (p:stmt) -> (s0:state) -> (s1:state) -> Type0 =
 //   runsto (IfZ c (Seq b (While c b)) Skip) s s' ->
 //   runsto (While c b) s s'
 let r_while (#c:expr) (#b:stmt) (#s #s' : state) (pf : runsto (IfZ c (Seq b (While c b)) Skip) s s')
-  : runsto (While c b) s s'
-= admit()
+  : runsto (While c b) s s' =
+  match pf with
+  | R_IfZ_False pfe ec ->
+    R_While_False ec
+
+  | R_IfZ_True pft ec ->
+    let R_Seq rp rq = pft in
+    R_While_True rp ec rq
 
 type cond = state -> bool
 
 noeq
 type hoare : (pre:cond) -> (p:stmt) -> (post:cond) -> Type0 =
   | H_Skip : pre:cond -> hoare pre Skip pre // {P} Skip {P}
+
   | H_Seq :
     #p:stmt -> #q:stmt ->
     #pre:cond -> #mid:cond -> #post:cond ->
     hoare pre p mid -> hoare mid q post ->
     hoare pre (Seq p q) post  // {pre} p {mid} /\ {mid} q {post}    ==>    {pre} p;q {post}
 
+  | H_IfZ :
+    #c:expr -> #t:stmt -> #e:stmt ->
+    #pre:cond -> #post:cond ->
+    hoare (fun s -> pre s && eval_expr s c = 0) t post ->  // {pre /\ c = 0} t {post} /\
+    hoare (fun s -> pre s && eval_expr s c <> 0) e post -> // {pre /\ c <> 0} e {post} ==>
+    hoare pre (IfZ c t e) post                             // {pre} if c then t else e {post}
+
+  | H_Assign :
+    #x:var -> #e:expr ->
+    #pre:cond ->
+    hoare (fun s -> pre (override s x (eval_expr s e))) (Assign x e) pre // {pre /\ x = e} x := e {pre}
+
+  | H_While :
+    #c:expr -> #b:stmt ->
+    #inv:cond ->
+    hoare (fun s -> inv s && eval_expr s c = 0) b inv ->         // {inv /\ c = 0} b {inv} ==>
+    hoare inv (While c b) (fun s -> inv s && eval_expr s c <> 0) // {inv} while c b {inv /\ c <> 0}
+
 let rec hoare_ok (p:stmt) (pre:cond) (post:cond) (pf : hoare pre p post)
                  (s0 s1 : state) (e_pf : runsto p s0 s1)
   : Lemma (requires pre s0)
           (ensures  post s1)
-= admit()
+= match pf with
+
+  | H_Seq #p #q #pre #mid #post hp hq ->
+    let R_Seq #p #q #s0 #sint #s1 rp rq = e_pf in
+    hoare_ok p pre mid hp s0 sint rp;
+    hoare_ok q mid post hq sint s1 rq
+
+  | H_IfZ ht he ->
+    begin
+      match e_pf with
+      | R_IfZ_False #c #t #e #s0 #s1 re ec ->
+        hoare_ok e (fun s -> pre s && eval_expr s c <> 0) post he s0 s1 re
+
+      | R_IfZ_True #c #t #e #s0 #s1 rt ec ->
+        hoare_ok t (fun s -> pre s && eval_expr s c = 0) post ht s0 s1 rt
+    end
+  
+  | H_While #c #b #inv hb ->
+    begin
+      match e_pf with
+      | R_While_True #c #b #s0 #sint #s1 rb ec rw ->
+        hoare_ok b (fun s -> inv s && eval_expr s c = 0) inv hb s0 sint rb;
+        hoare_ok (While c b) inv (fun s -> inv s && eval_expr s c <> 0) pf sint s1 rw
+
+      | _ -> ()
+    end
+
+  | _ -> ()
 
 let st0 : state = fun _ -> 0
 
-let test1 : hoare (fun _ -> true) (Assign "x" (Const 1)) (fun s -> s "x" = 1) =
-  admit()
+let test1 : hoare (fun _ -> true) (Assign "x" (Const 1)) (fun s -> s "x" = 1) = H_Assign
